Cappy/Translation/Encoding/CaptureSet/Properties.lean
@@ -1,4 +1,9 @@
 import Cappy.Translation.Encoding.CaptureSet.Core
 namespace Cappy
 
+theorem CaptureSet.interp_inj
+  (hi1 : CaptureSet.Interp ρ Γ C D I1)
+  (hi2 : CaptureSet.Interp ρ Γ C D I2) :
+  I1 = I2 := sorry
+
 end Cappy
